

# Replication Exercise -Set Identification, Mrs

Jordi Torres

December 18, 2025

## Exercise 1

- We can interpret  $\beta_l$  as the increase in production given an increase in labor, keeping prices fixed. Derivation in section 1
- Now we need to assume that both inputs are flexible and static. This is totally unrealistic for capital, as it is quite unlikely that farmers invest in capital non-dynamically (tools/machines last periods, 1920..old technology, even more) and that can quickly adjust their levels of capital in the short run. I derive results in section 1
- 

## 1 Appendix

### 1

Under perfect competition and one mobile input only (labor) we have that the firm solves:

$$\begin{aligned} \min_{L_{f,t}, K_{f,t} \geq 0} \quad & L_{f,t}W_{f,t} + K_{f,t}R_{f,t} \\ \text{s.t.} \quad & \bar{Q}_{f,t} = L_{f,t}^{\beta_l} K_{f,t}^{\beta_k} \Omega_{f,t} \end{aligned}$$

From the first order condition on labor:

$$W_{f,t} = \lambda \beta_l \left( \frac{Q_{f,t}}{L_{f,t}} \right)$$

By definition:  $\mu_{f,t} = \frac{p_{f,t}}{\lambda_{f,t}}$

$$W_{f,t} = \frac{p_{f,t}}{\mu_{f,t}} \beta_l \left( \frac{Q_{f,t}}{L_{f,t}} \right)$$

Under perfect competition  $\mu_{f,t}=1$ , then rearranging we get:

$$\beta_l = \frac{W_{f,t} L_{f,t}}{P_{f,t} Q_{f,t}}$$

Which we can estimate with a simple average.

### Text B

From the same problem above, if we take first order conditions with respect to labor and capital we get:

$$W_{f,t} L_{f,t} = \lambda \beta_l (Q_{f,t})$$

$$R_{f,t} K_{f,t} = \lambda \beta_k (Q_{f,t})$$

If we sum the two expressions:  $W_{f,t} L_{f,t} + R_{f,t} K_{f,t} = \lambda \beta_l (Q_{f,t}) + \lambda \beta_k (Q_{f,t})$

which reduces to:

$$W_{f,t} L_{f,t} + R_{f,t} K_{f,t} = \lambda Q_{f,t}$$

Then if we take 1 or 2 and divide by the same in both sides:

$$\frac{W_{f,t} L_{f,t}}{W_{f,t} L_{f,t} + R_{f,t} K_{f,t}} = \frac{\lambda \beta_l (Q_{f,t})}{\lambda Q_{f,t}}$$

This simplifies:  $\frac{W_{f,t} L_{f,t}}{W_{f,t} L_{f,t} + R_{f,t} K_{f,t}} = \beta_l$

Same argument for the other. The markup also comes from the expression from above:

$\lambda = \frac{W_{f,t} L_{f,t}}{Q_{f,t} \beta_l}$  If we substitute  $\beta_l$  into this expression and we rearrange we have:

$$\lambda = \frac{W_{f,t} L_{f,t} + R_{f,t} K_{f,t}}{Q_{f,t}}$$

Thus:  $\mu = \frac{p Q_{f,t}}{W_{f,t} L_{f,t} + R_{f,t} K_{f,t}}$

